Progress on commutation theorems
But some of them are the wrong ones :-/

common/ModuleSemantics.v
@@ -15,7 +15,7 @@ Require Import Sets.
   then the flat composition will handle it in a similar way. However,
   the components cannot call each other. *)
 
-Module FComp.
+Module SFComp.
   Section FLATCOMP.
     Context (ge: Senv.t).
     Context {li} (L1 L2: semantics li).
@@ -23,20 +23,15 @@ Module FComp.
     Definition genv: Type := genvtype L1 * genvtype L2.
 
     Inductive state {A B} :=
-      | running (s: A + B) (k: cont li (A + B))
+      | state_l (s: A) (k: cont li B)
+      | state_r (s: B) (k: cont li A)
       | conflict.
 
-    Definition inlk {A B} (k: cont li A) : cont li (A + B) :=
-      fun q => option_map (set_map inl) (k q).
-
-    Definition inrk {A B} (k: cont li B) : cont li (A + B) :=
-      fun q => option_map (set_map inr) (k q).
-
-    Definition liftk {A B} (k1 k2: cont li (A + B)): cont li state :=
+    Definition liftk {A B} (k1: cont li A) (k2: cont li B): cont li state :=
       fun q =>
         match k1 q, k2 q with
-          | Some S1, None => Some (set_map (fun S => running S k2) S1)
-          | None, Some S2 => Some (set_map (fun S => running S k1) S2)
+          | Some S1, None => Some (set_map (fun S => state_l S k2) S1)
+          | None, Some S2 => Some (set_map (fun S => state_r S k1) S2)
           | Some _, Some _ => Some (singl conflict)
           | None, None => None
         end.
@@ -44,23 +39,23 @@ Module FComp.
     Inductive step (ge: genv): state -> trace -> state -> Prop :=
       | step_l s t s' k:
           Smallstep.step L1 (fst ge) s t s' ->
-          step ge (running (inl s) k) t (running (inl s') k)
+          step ge (state_l s k) t (state_l s' k)
       | step_r s t s' k:
           Smallstep.step L2 (snd ge) s t s' ->
-          step ge (running (inr s) k) t (running (inr s') k).
+          step ge (state_r s k) t (state_r s' k).
 
     Definition initial_state: cont li state :=
       liftk
-        (inlk (initial_state L1))
-        (inrk (initial_state L2)).
+        (initial_state L1)
+        (initial_state L2).
 
     Inductive final_state: state -> reply li -> _ -> Prop :=
-      | final_state_l s1 r1 k1 k':
-          Smallstep.final_state L1 s1 r1 k1 ->
-          final_state (running (inl s1) k') r1 (liftk (inlk k1) k')
-      | final_state_r s2 r2 k2 k':
-          Smallstep.final_state L2 s2 r2 k2 ->
-          final_state (running (inr s2) k') r2 (liftk (inrk k2) k').
+      | final_state_l s r k k':
+          Smallstep.final_state L1 s r k ->
+          final_state (state_l s k') r (liftk k k')
+      | final_state_r s r k k':
+          Smallstep.final_state L2 s r k ->
+          final_state (state_r s k') r (liftk k' k).
 
     Definition semantics :=
       {|
@@ -73,7 +68,7 @@ Module FComp.
         Smallstep.symbolenv := ge;
       |}.
     End FLATCOMP.
-End FComp.
+End SFComp.
 
 (** * Resolution operator *)
 
@@ -87,7 +82,7 @@ End FComp.
   initially wrong, this behavior would be cancelled out by the
   alternative step. *)
 
-Module Res.
+Module SRes.
   Section RESOLVE.
     Context {li} (sw: reply li -> query li) (L: Smallstep.semantics li).
 
@@ -116,14 +111,14 @@ Module Res.
         Smallstep.symbolenv := symbolenv L;
       |}.
   End RESOLVE.
-End Res.
+End SRes.
 
 (** * Horizontal composition *)
 
 (** Applying the resolution operator to the flat composition of
   some transitions systems gives us horizontal composition. *)
 
-Module HComp.
+Module SHComp.
   Section HCOMP.
     Context (ge: Senv.t).
     Context {li} (L1 L2: semantics (li -o li)).
@@ -135,6 +130,6 @@ Module HComp.
       end.
 
     Definition semantics :=
-      Res.semantics sw (FComp.semantics ge L1 L2).
+      SRes.semantics sw (SFComp.semantics ge L1 L2).
   End HCOMP.
-End HComp.
+End SHComp.
